added second freelist to make allocator closer to a page in mimalloc

misc-verification/slab_allocator.v
@@ -10,15 +10,16 @@ Definition freelist_push : val := λ: "fl" "l",
   "l" <- !"fl" ;; 
   "fl" <- SOME "l".
 
-Definition new_alloc_lazy : val := λ: "n" "bs", 
-  let: "al" := AllocN ("n" * "bs" + #4) NONE in 
+Definition new_alloc : val := λ: "n" "bs", 
+  let: "al" := AllocN ("n" * "bs" + #5) NONE in 
   "al" <- NONE ;;
-  "al" +ₗ #1 <- "n" ;;
-  "al" +ₗ #2 <- #0 ;;
-  "al" +ₗ #3 <- "bs" ;;
+  "al" +ₗ #1 <- NONE ;;
+  "al" +ₗ #2 <- "n" ;;
+  "al" +ₗ #3 <- #0 ;;
+  "al" +ₗ #4 <- "bs" ;;
   "al".
 
-Definition free : val := λ: "al" "l", freelist_push "al" "l".
+Definition free : val := λ: "al" "l", freelist_push ("al" +ₗ #1) "l".
 
 Definition freelist_extend : val := rec: "rec" "fl" "lb" "bs" "n" "c" :=
   if: "c" + #1 ≤ "n"
@@ -28,20 +29,27 @@ Definition freelist_extend : val := rec: "rec" "fl" "lb" "bs" "n" "c" :=
   
 Definition extend : val := λ: "al", 
   let: "fl" := "al" in
-  let: "res" := !("al" +ₗ #1) in 
-  let: "cap" := !("al" +ₗ #2) in 
-  let: "bs" := !("al" +ₗ #3) in
+  let: "res" := !("al" +ₗ #2) in 
+  let: "cap" := !("al" +ₗ #3) in 
+  let: "bs" := !("al" +ₗ #4) in
   let: "mext" := if: "cap" = #0 then #1 else "cap" in
   let: "ext" := if: "mext" ≤ "res" - "cap" then "mext" else "res" - "cap" in 
   if: "ext" = #0 then NONE 
   else 
-  freelist_extend "fl" ("al" +ₗ (#4 + "cap" * "bs")) "bs" ("ext" - #1) #0 ;;
-    ("al" +ₗ #2) <- ("cap" + "ext") ;;
-    SOME ("al" +ₗ (#4 + ("cap" + "ext" - #1) * "bs")).
+  freelist_extend "fl" ("al" +ₗ (#5 + "cap" * "bs")) "bs" ("ext" - #1) #0 ;;
+    ("al" +ₗ #3) <- ("cap" + "ext") ;;
+    SOME ("al" +ₗ (#5 + ("cap" + "ext" - #1) * "bs")).
 
 Definition alloc : val := λ: "al", 
   match: freelist_pop "al" with 
-    NONE => extend "al" 
+    NONE => 
+      match: freelist_pop ("al" +ₗ #1) with 
+        NONE => extend "al" 
+      | SOME "l" => 
+        "al" <- !("al" +ₗ #1) ;;
+        "al" +ₗ #1 <- NONE ;;
+        SOME "l"
+        end
   | SOME "l" => SOME "l"
   end.
   
@@ -53,87 +61,90 @@ Section Hoare.
   Implicit Types v w : val.
   
   Definition is_valid_loc l al : iProp Σ := 
-    ∃ (res bs i : nat), (al +ₗ 1) ↦□ #res ∗ (al +ₗ 3) ↦□ #bs ∗ 
-      ⌜l = (al +ₗ (4 + i * bs))⌝ ∗ ⌜i < res⌝.
+    ∃ (res bs i : nat), (al +ₗ 2) ↦□ #res ∗ (al +ₗ 4) ↦□ #bs ∗ 
+      ⌜l = (al +ₗ (5 + i * bs))⌝ ∗ ⌜i < res⌝.
 
   Global Instance is_valid_loc_presist l al : Persistent (is_valid_loc l al).
   Proof. apply _. Qed.
 
   Fixpoint is_freelist_rec l al size : iProp Σ := 
-    ∃ bs, (al +ₗ 3) ↦□  #(S bs) ∗
+    ∃ bs, (al +ₗ 4) ↦□  #(S bs) ∗
     match size with 
     | O => l ↦ NONEV ∗ ([∗ list] i ∈ seq 1 bs, ∃ v, (l +ₗ i) ↦  v) ∗ is_valid_loc l al 
     | S s => ∃ l1, l ↦ SOMEV #l1 ∗ ([∗ list] i ∈ seq 1 bs, ∃ v, (l +ₗ i) ↦  v) ∗
           is_valid_loc l al ∗ is_freelist_rec l1 al s
     end.
     
-  Definition is_freelist al : iProp Σ := 
-    al ↦ NONEV 
+  Definition is_freelist fl al : iProp Σ := 
+    fl ↦ NONEV 
       ∨
-    ∃ l1 size, al ↦ SOMEV #l1 ∗ is_freelist_rec l1 al size.
+    ∃ l1 size, fl ↦ SOMEV #l1 ∗ is_freelist_rec l1 al size.
 
+  (*might not want bs to be persistant as mimalloc can repurpose a  
+     page to new page queue so new size *)
   Definition is_allocator (al : loc) bs : iProp Σ := 
-    ∃ (res cap : nat), ⌜res > 0⌝ ∗ ⌜cap ≤ res⌝ ∗ ⌜bs > 0⌝ ∗ (al +ₗ 1) ↦□  #res ∗ 
-      (al +ₗ 2) ↦ #cap ∗ (al +ₗ 3) ↦□  #bs ∗ is_freelist al ∗  
-      (al +ₗ (4 + cap * bs)) ↦∗ replicate ((res - cap) * bs) NONEV. 
+    ∃ (res cap : nat), ⌜res > 0⌝ ∗ ⌜cap ≤ res⌝ ∗ ⌜bs > 0⌝ ∗ (al +ₗ 2) ↦□  #res ∗ 
+      (al +ₗ 3) ↦ #cap ∗ (al +ₗ 4) ↦□  #bs ∗ is_freelist al al ∗ 
+      is_freelist (al +ₗ 1) al ∗
+      (al +ₗ (5 + cap * bs)) ↦∗ replicate ((res - cap) * bs) NONEV. 
 
   Lemma new_alloc_hoare res bs : 
     {{{ ⌜res > 0⌝ ∗ ⌜bs > 0⌝ }}} 
-      new_alloc_lazy #res #bs 
+      new_alloc #res #bs 
     {{{ al, RET #al; is_allocator al bs }}}.
   Proof. 
-    iIntros (φ) "(%Hn & %Hbs) Hphi". iUnfold new_alloc_lazy. wp_pures.
+    iIntros (φ) "(%Hn & %Hbs) Hphi". iUnfold new_alloc. wp_pures.
     wp_apply wp_allocN; [lia|done|]. iIntros "%al (HalN & _)". 
-    assert (Heq : Z.to_nat (res * bs + 4) = S (S (S (S (res * bs))))) by lia.
-    rewrite Heq. simpl. rewrite 4!array_cons.
-    iDestruct "HalN" as "(Hal & Hal1 & Hal2 & Hal3 & HalN)". wp_store. wp_store.
-    rewrite 3!Loc.add_assoc. wp_store. wp_store. iApply "Hphi". 
+    assert (Heq : Z.to_nat (res * bs + 5) = S (S (S (S (S (res * bs)))))) by lia.
+    rewrite Heq. simpl. rewrite 5!array_cons.
+    iDestruct "HalN" as "(Hal & Hal1 & Hal2 & Hal3 & Hal4 & HalN)". wp_store. 
+    wp_store. rewrite !Loc.add_assoc. wp_store. wp_store. wp_store. iApply "Hphi". 
     iExists res, 0. 
-    iMod (pointsto_persist with "Hal1") as "#Hal1". 
-    iMod (pointsto_persist with "Hal3") as "#Hal3". iFrame "Hal Hal1 Hal2 Hal3".
+    iMod (pointsto_persist with "Hal2") as "#Hal2". 
+    iMod (pointsto_persist with "Hal4") as "#Hal4". iFrame "Hal Hal1 Hal2 Hal3 Hal4".
     iSplitR; [by iPureIntro|]. iSplitR; [iPureIntro; lia|]. iSplitR; [by iPureIntro|]. 
     by rewrite Z.mul_0_l Nat.sub_0_r.
   Qed.
 
-  Lemma freelist_pop_hoare al bs : 
-    {{{ (al +ₗ 3) ↦□ #bs ∗ is_freelist al }}} 
-      freelist_pop #al
+  Lemma freelist_pop_hoare al fl bs : 
+    {{{ (al +ₗ 4) ↦□ #bs ∗ is_freelist fl al }}} 
+      freelist_pop #fl
     {{{ vret, RET vret; 
-      is_freelist al ∗
-      (⌜vret = NONEV⌝ 
+      (⌜vret = NONEV⌝ ∗ fl ↦ NONEV 
         ∨ 
       ∃ l, ⌜vret = SOMEV #l⌝ ∗ 
-        ([∗ list] i ∈ seq 0 bs, ∃ v, (l +ₗ i) ↦ v) ∗ is_valid_loc l al)
+        ([∗ list] i ∈ seq 0 bs, ∃ v, (l +ₗ i) ↦ v) ∗ 
+        is_valid_loc l al ∗ is_freelist fl al)
     }}}. 
   Proof.
-    iIntros (φ) "(#Hal3 & [H | (%l1 & %s & Hfl & Hflr)]) Hphi"; 
+    iIntros (φ) "(#Hal4 & [H | (%l1 & %s & Hfl & Hflr)]) Hphi"; 
     iUnfold freelist_pop; wp_load; wp_pures.
     { iApply "Hphi". iFrame. by iLeft. }
     destruct s; simpl.
-    { iDestruct "Hflr" as "(%bs1 & #Hal3' & Hl1 & Hl1r & #Hl1v)". 
+    { iDestruct "Hflr" as "(%bs1 & #Hal4' & Hl1 & Hl1r & #Hl1v)". 
       wp_load. wp_store. wp_pures. iApply "Hphi". iFrame. iRight. 
       iExists l1. iFrame. iSplitR; [by iPureIntro|].
-      iCombine "Hal3 Hal3'" gives %[_ Heq]. simplify_eq. simpl. iFrame "Hl1v Hl1r". 
+      iCombine "Hal4 Hal4'" gives %[_ Heq]. simplify_eq. simpl. iFrame "Hl1v Hl1r". 
       iExists NONEV. by rewrite Loc.add_0. }
-    iDestruct "Hflr" as "(%bs1 & #Hal3' & %l & Hl1 & Hl1r & #Hl1v & Hflr)". 
+    iDestruct "Hflr" as "(%bs1 & #Hal4' & %l & Hl1 & Hl1r & #Hl1v & Hflr)". 
     wp_load. wp_store. wp_pures. iApply "Hphi". 
-    iSplitL "Hfl Hflr"; [iRight; by iFrame|]. iRight.     
-    iCombine "Hal3 Hal3'" gives %[_ Heq]. simplify_eq. simpl. iFrame "Hl1v Hl1r". 
-    iSplitR; [by iPureIntro|]. rewrite Loc.add_0. auto. 
+    iRight. iCombine "Hal4 Hal4'" gives %[_ Heq]. simplify_eq. simpl. 
+    iFrame "Hl1v Hl1r". iSplitR; [by iPureIntro|]. rewrite Loc.add_0. 
+    iSplitL "Hl1"; [auto|]. iRight. by iFrame. 
   Qed.
 
-  Lemma freelist_push_hoare l al : 
+  Lemma freelist_push_hoare l fl al : 
     {{{ 
-      ∃ bs, (al +ₗ 3) ↦□ #(S bs) ∗
-      is_freelist al ∗ (([∗ list] i ∈ seq 0 (S bs), ∃ v, (l +ₗ i) ↦ v)) ∗ 
+      ∃ bs, (al +ₗ 4) ↦□ #(S bs) ∗
+      is_freelist fl al ∗ (([∗ list] i ∈ seq 0 (S bs), ∃ v, (l +ₗ i) ↦ v)) ∗ 
       is_valid_loc l al 
     }}}
-      freelist_push #al #l
-    {{{ RET #(); is_freelist al }}}.
+      freelist_push #fl #l
+    {{{ RET #(); is_freelist fl al }}}.
   Proof. 
-    simpl. rewrite Loc.add_0. iIntros (φ) "(%bs&#Hal3&[H | (%l1 & %s & Hfl & Hflr)] & 
+    simpl. rewrite Loc.add_0. iIntros (φ) "(%bs&#Hal4&[H | (%l1 & %s & Hfl & Hflr)] & 
     ((%v & Hl) & Hl1bs) & Hlv) Hphi"; iUnfold freelist_push; wp_load; wp_store; 
-    wp_store. { iApply "Hphi". iRight. iFrame. iExists 0. iFrame. by iFrame "Hal3". }
+    wp_store. { iApply "Hphi". iRight. iFrame. iExists 0. iFrame. by iFrame "Hal4". }
     iApply "Hphi". iRight. iExists l, (S s). by iFrame. 
   Qed.
 
@@ -145,10 +156,10 @@ Section Hoare.
       free #al #l
     {{{ RET #(); is_allocator al (S bs) }}}.
   Proof.
-    iIntros (φ) "((%res&%cap&%Hr&%Hcr&%Hbs&#Hal1&Hal2&#Hal3&Hfl&Hun) &Hlbs&#Hlv) Hphi".
-    iUnfold free. wp_pures. iApply (freelist_push_hoare with "[Hfl Hlbs]").
-    - iFrame. iFrame "Hlv Hal3".
-    - iNext. iIntros "Hfl". iApply "Hphi". iFrame. auto.
+    iIntros (φ) "((%res&%cap&%Hr&%Hcr&%Hbs&#Hal2&Hal3&#Hal4&Hfl&Hfl2&Hun)&Hlbs&#Hlv)Hphi".
+    iUnfold free. wp_pures. iApply (freelist_push_hoare with "[Hfl2 Hlbs]").
+    - iFrame. auto. 
+    - iNext. iIntros "Hfl2". iApply "Hphi". iFrame. auto.
   Qed.
 
   Lemma seq_array_pointsto_eq l dq v n :
@@ -162,21 +173,21 @@ Section Hoare.
     setoid_rewrite <-Loc.add_assoc; iApply "IH"; done.
   Qed.
 
-  Lemma freelist_extend_hoare al res bs lb cap n c d : 
+  Lemma freelist_extend_hoare fl al res bs lb cap n c d : 
     d = n - c -> 
-    lb = (al +ₗ (4 + cap * bs)) ->
+    lb = (al +ₗ (5 + cap * bs)) ->
     cap ≤ res ->
     n ≤ res - cap ->
     bs > 0 ->
     {{{ 
-      (al +ₗ 1) ↦□ #res ∗ (al +ₗ 3) ↦□ #bs ∗
-      is_freelist al ∗ (lb +ₗ (c * bs)) ↦∗ replicate (d * bs) NONEV 
+      (al +ₗ 2) ↦□ #res ∗ (al +ₗ 4) ↦□ #bs ∗
+      is_freelist fl al ∗ (lb +ₗ (c * bs)) ↦∗ replicate (d * bs) NONEV 
     }}} 
-      freelist_extend #al #lb #bs #n #c
-    {{{ RET #(); is_freelist al }}}. 
+      freelist_extend #fl #lb #bs #n #c
+    {{{ RET #(); is_freelist fl al }}}. 
   Proof. 
     iInduction d as [|d IH] forall (c); simpl; 
-    iIntros (Hd -> Hcr Hd2 Hbs φ) "(#Hal1 & #Hal3 & Hfl & Hun) Hphi"; 
+    iIntros (Hd -> Hcr Hd2 Hbs φ) "(#Hal2 & #Hal4 & Hfl & Hun) Hphi"; 
     iUnfold freelist_extend; wp_pures. 
     { case_bool_decide; [lia|]. wp_pures. by iApply "Hphi". }
     case_bool_decide; [|lia]. wp_pures. 
@@ -184,7 +195,7 @@ Section Hoare.
     iDestruct "Hun" as "(Hun1 & Hun2)". 
     wp_apply (freelist_push_hoare with "[Hfl Hun1]").
     { iFrame "Hfl". iExists (bs - 1). assert (S (bs - 1) = bs) by lia. rewrite H0.
-      iFrame "Hal3 Hal1". iSplitL "Hun1". 
+      iFrame "Hal4 Hal2". iSplitL "Hun1". 
       - Search "↦∗" replicate. iApply big_sepL_mono; 
         [|iApply seq_array_pointsto_eq; iApply "Hun1"]. iIntros. auto.
       - iExists (cap + c). iPureIntro. split; [|lia]. rewrite Loc.add_assoc. 
@@ -193,7 +204,7 @@ Section Hoare.
     assert (Heq : (Z.of_nat c + 1)%Z = Z.of_nat (c + 1)) by lia. rewrite Heq. 
     iApply ("IH" with "[] [] [] [] [] [Hfl Hun2]"); try iPureIntro; 
     [lia|done|lia|lia|done| |]. 
-    { iFrame "Hal1 Hal3 Hfl". rewrite Loc.add_assoc. 
+    { iFrame "Hal2 Hal4 Hfl". rewrite Loc.add_assoc. 
       by rewrite Nat2Z.inj_add Z.mul_add_distr_r Z.mul_1_l. }
     iNext. iIntros. by iApply "Hphi".
   Qed. 
@@ -209,23 +220,22 @@ Section Hoare.
         ⌜vret = NONEV⌝)
       }}}.
   Proof. 
-    iIntros (φ) "(%res&%cap&%Hr&%Hcr&%Hbs&#Hal1&Hal2&#Hal3&Hfl&Hun) Hphi". 
+    iIntros (φ) "(%res&%cap&%Hr&%Hcr&%Hbs&#Hal2&Hal3&#Hal4&Hfl&Hfl2&Hun) Hphi". 
     iUnfold extend. wp_pures. wp_load. wp_load. wp_load. wp_pures. 
     destruct (decide (cap = 0)) as [Hc | Hc]. 
     { rewrite Hc. wp_pures. case_bool_decide; [|lia]. wp_pures. 
-      wp_apply ((freelist_extend_hoare al res bs (al +ₗ 4) 0 0 0 0) with "[Hfl]"); 
-      try lia; [by rewrite Z.mul_0_l|rewrite array_nil; iFrame "Hal1 Hal3 Hfl"|].
-      rewrite Nat.sub_0_r. destruct res; [lia|]. simpl. 
+      wp_apply ((freelist_extend_hoare al al res bs (al +ₗ 5) 0 0 0 0) with "[Hfl]"); 
+      try lia; [by rewrite Z.mul_0_l|rewrite array_nil; iFrame "Hal2 Hal4 Hfl"|].
+      rewrite Nat.sub_0_r Z.mul_0_l. destruct res; [lia|]. simpl. 
       rewrite replicate_add array_app. iDestruct "Hun" as "(Hun1 & Hun2)". 
-      iIntros "Hfl". wp_store. wp_pures. iApply "Hphi". iSplitL "Hal2 Hun2 Hfl".
-      { rewrite length_replicate Z.add_0_l. iFrame "Hal3 Hal1 Hfl". 
-        iExists 1. iFrame "Hal2". iSplitR; [by iPureIntro|]. iSplitR; 
+      iIntros "Hfl". wp_store. wp_pures. iApply "Hphi". iSplitL "Hal3 Hun2 Hfl Hfl2".
+      { rewrite length_replicate Z.add_0_l Z.add_0_r Loc.add_assoc. 
+        iFrame "Hal2 Hal4 Hfl Hfl2". iExists 1. iSplitR; [by iPureIntro|]. iSplitR; 
         [iPureIntro; lia|]. iSplitR; [by iPureIntro|]. assert (S res - 1 = res) by lia.
-        by rewrite Z.mul_0_l Z.mul_1_l Loc.add_assoc H0. }
-      iLeft. rewrite Z.mul_0_l !Z.add_0_r. iExists (al +ₗ 4). iSplitR; [done|].
-      iSplitL.
+        rewrite Z.mul_1_l H0. by iSplitL "Hal3". }
+      iLeft. rewrite Z.mul_0_l !Z.add_0_r. iExists _. iSplitR; [done|]. iSplitL.
       { iApply big_sepL_mono; [|by iApply seq_array_pointsto_eq]. iIntros. auto. }
-      iFrame "Hal3 Hal1". iExists 0. rewrite Z.mul_0_l. iPureIntro. split; [done|lia]. }
+      iFrame "Hal4 Hal2". iExists 0. rewrite Z.mul_0_l. iPureIntro. split; [done|lia]. }
     case_bool_decide; [inv H; lia|]. wp_pures. case_bool_decide.
     { wp_pures. case_bool_decide; [inv H1; lia|]. wp_pures. 
       assert (Z.of_nat (cap - 1) = (Z.of_nat cap - 1)%Z) by lia. rewrite -H2.
@@ -233,60 +243,60 @@ Section Hoare.
       assert ((res - cap) * bs = (cap - 1) * bs + (res - cap - (cap - 1)) * bs) 
       by lia. rewrite H3 replicate_add array_app. 
       iDestruct "Hun" as "(Hun1 & Hun2)". rewrite length_replicate.
-      wp_apply (freelist_extend_hoare al res bs (al +ₗ (4 + (cap * bs))) cap 
+      wp_apply (freelist_extend_hoare al al res bs (al +ₗ (5 + (cap * bs))) cap 
       (cap - 1) 0 (cap - 1) with "[Hfl Hun1]"); try lia; [done| |].
-      { iFrame "Hal1 Hfl Hal3". by rewrite Z.mul_0_l Loc.add_0. }
+      { iFrame "Hal2 Hfl Hal4". by rewrite Z.mul_0_l Loc.add_0. }
       iIntros "Hfl". wp_store. wp_pures. iApply "Hphi".  
       (*split: bs of *)
       assert (res - cap - (cap - 1) = 1 + (res - cap - cap)) by lia. rewrite H4.
       rewrite Nat.mul_add_distr_r Nat.mul_1_l replicate_add array_app.
       iDestruct ("Hun2") as "(Hun1 & Hun2)". iSplitR "Hun1". 
-      { rewrite -Nat2Z.inj_add. iFrame "Hal1 Hal3 Hal2 Hfl". iSplitR; [by iPureIntro|].
-        iSplitR; [iPureIntro; lia|]. iSplitR; [by iPureIntro|]. 
+      { rewrite -Nat2Z.inj_add. iFrame "Hal2 Hal3 Hal4 Hfl Hfl2". iSplitR; 
+        [by iPureIntro|]. iSplitR; [iPureIntro; lia|]. iSplitR; [by iPureIntro|]. 
         rewrite length_replicate !Loc.add_assoc. 
-        assert ((4 + cap * bs + (((cap - 1) * bs)%nat + bs))%Z 
-        = (4 + (cap + cap)%nat * bs)%Z) by lia.
+        assert ((5 + cap * bs + (((cap - 1) * bs)%nat + bs))%Z 
+        = (5 + (cap + cap)%nat * bs)%Z) by lia.
         assert ((res - cap - cap) * bs = (res - (cap + cap)) * bs) by lia.
         by rewrite H5 H6. }
       iLeft. rewrite Loc.add_assoc. 
-      assert ((4 + (cap + cap - 1) * bs)%Z = 
-      4 + cap * bs + ((cap - 1) * bs)%nat) by lia. rewrite H5. iExists _. 
+      assert ((5 + (cap + cap - 1) * bs)%Z = 
+      5 + cap * bs + ((cap - 1) * bs)%nat) by lia. rewrite H5. iExists _. 
       iSplitR; [by iPureIntro|]. iSplitL. 
       { iApply big_sepL_mono; [|iApply seq_array_pointsto_eq; iApply "Hun1"].
         iIntros. iExists NONEV. 
-        assert ((4 + cap * bs + ((cap - 1) * bs)%nat)%Z = 
-        (4 + cap * bs + (cap - 1) * bs)%nat) by lia. by rewrite H7.  }
-      iFrame "Hal1 Hal3". iExists (cap + (cap - 1)). iPureIntro.
+        assert ((5 + cap * bs + ((cap - 1) * bs)%nat)%Z = 
+        (5 + cap * bs + (cap - 1) * bs)%nat) by lia. by rewrite H7.  }
+      iFrame "Hal2 Hal4". iExists (cap + (cap - 1)). iPureIntro.
       split; [|lia]. f_equal. lia. } 
     wp_pures. destruct (decide (res - cap = 0)) as [Hcr2 | Hcr2]. 
     { rewrite -Nat2Z.inj_sub; [|done]. rewrite Hcr2. wp_pures. 
       iApply "Hphi". iSplitL; [|by iRight].
-      iFrame "Hal1 Hal3 Hal2 Hfl". iSplitR; [by iPureIntro|]. 
+      iFrame "Hal2 Hal3 Hal4 Hfl Hfl2". iSplitR; [by iPureIntro|]. 
       iSplitR; [by iPureIntro|]. iSplitR; [by iPureIntro|]. by rewrite Hcr2. }
     case_bool_decide; [inv H1; lia|]. wp_pures.
     (* split (res - cap - 1) * bs + bs  *)
     assert (res - cap = (res - cap - 1) + 1) by lia. rewrite H2. 
     rewrite Nat.mul_add_distr_r Nat.mul_1_l replicate_add array_app length_replicate. 
     iDestruct "Hun" as "(Hun1 & Hun2)". 
-    iPoseProof (freelist_extend_hoare al res bs (al +ₗ (4 + cap * bs)) 
+    iPoseProof (freelist_extend_hoare al al res bs (al +ₗ (5 + cap * bs)) 
     cap (res - cap - 1) 0 (res - cap - 1)) as "H"; [lia|done|done|lia|done|]. 
     assert (Z.of_nat (res - cap - 1) = (Z.of_nat res - Z.of_nat cap - 1)%Z) by lia.
     rewrite H3. wp_apply ("H" with "[Hfl Hun1]"). 
-    { rewrite Loc.add_assoc Z.mul_0_l Z.add_0_r. iFrame "Hfl Hun1 Hal1 Hal3". }
+    { rewrite Loc.add_assoc Z.mul_0_l Z.add_0_r. iFrame "Hfl Hun1 Hal2 Hal4". }
     iIntros "Hfl". wp_store. wp_pures. iApply "Hphi". 
     (* split bs of*) 
-    iSplitL "Hfl Hal2". 
+    iSplitL "Hfl Hfl2 Hal3". 
     { rewrite -Nat2Z.inj_sub; [|done]. rewrite -Nat2Z.inj_add. 
-      iFrame "Hal1 Hal2 Hal3 Hfl". iSplitR; [by iPureIntro|]. iSplitR; 
+      iFrame "Hal2 Hal3 Hal4 Hfl Hfl2". iSplitR; [by iPureIntro|]. iSplitR; 
       [iPureIntro; lia|]. iSplitR; [by iPureIntro|].
       assert (res - (cap + (res - cap)) = 0) by lia. rewrite H4 Nat.mul_0_l.
       simpl. by rewrite array_nil. }
     iLeft. rewrite !Loc.add_assoc. 
-    assert ((4 + cap * bs + ((res - cap - 1) * bs)%nat)%Z 
-    = (4 + (cap + (res - cap) - 1) * bs)%Z) by lia. rewrite H4. 
+    assert ((5 + cap * bs + ((res - cap - 1) * bs)%nat)%Z 
+    = (5 + (cap + (res - cap) - 1) * bs)%Z) by lia. rewrite H4. 
     iExists _. iSplitR; [by iPureIntro|]. iSplitL.
     { iApply big_sepL_mono; [|by iApply seq_array_pointsto_eq]. iIntros. auto. }
-    iFrame "Hal1 Hal3". iExists (cap + (res - cap) - 1). iSplitR; [|iPureIntro; lia].
+    iFrame "Hal2 Hal4". iExists (cap + (res - cap) - 1). iSplitR; [|iPureIntro; lia].
     Set Printing Coercions. rewrite -Nat2Z.inj_sub; [|lia]. rewrite -Nat2Z.inj_add.
     assert ((Z.of_nat (cap + (res - cap)) - 1)%Z 
     = (Z.of_nat (cap + (res - cap) - 1))%Z) by lia. by rewrite H5. 
@@ -303,15 +313,24 @@ Section Hoare.
       ⌜vret = NONEV⌝)
     }}}.
   Proof.
-    iIntros (φ) "(%res&%cap&%Hr&%Hcr&%Hbs&#Hal1&Hal2&#Hal3&Hfl&Hun) Hphi". 
+    iIntros (φ) "(%res&%cap&%Hr&%Hcr&%Hbs&#Hal2&Hal3&#Hal4&Hfl&Hfl2&Hun) Hphi". 
     iUnfold alloc. wp_pures. 
-    wp_apply (freelist_pop_hoare with "[Hfl]"); [iFrame "Hfl Hal3"|].
-    iIntros (v) "(Hfl & [-> | (%l & -> & Hlbs & Hlv)])"; wp_pures.
-    { wp_apply (extend_hoare with "[Hal2 Hun Hfl]"); 
-      [iFrame "Hal1 Hal2 Hal3 Hfl Hun"; iPureIntro; lia|]. 
-      iIntros (v) "(Hal & [(%l & -> & Hlbs & Hlv) | ->])"; iApply "Hphi"; 
-      [iFrame; iLeft; iFrame; auto|iFrame; by iRight]. } 
-    iApply "Hphi". iFrame. iSplitR; [iFrame "Hal1 Hal3"; iPureIntro; lia|].
+    wp_apply (freelist_pop_hoare with "[Hfl]"); [iFrame "Hfl Hal4"|].
+    iIntros (v) "[(-> & Hfl) | (%l & -> & Hlbs & #Hlv & Hfl)]"; wp_pures.
+    { wp_apply (freelist_pop_hoare with "[Hfl2]"); [iFrame "Hfl2 Hal4"|].
+      iIntros (v) "[(-> & Hfl2) | (%l & -> & Hlbs & #Hlv & Hfl2)]"; wp_pures.
+      - wp_apply (extend_hoare with "[Hal3 Hun Hfl Hfl2]"); 
+        [iFrame "Hal2 Hal3 Hal4 Hfl2 Hfl Hun"; iPureIntro; lia|].
+        iIntros (v) "(Hal & [(%l & -> & Hlbs & #Hlv) | ->])"; iApply "Hphi"; 
+        [iFrame; iLeft; iFrame; auto|iFrame; by iRight]. 
+      - iDestruct "Hfl2" as "[Hal1 | (%l1 & %s1 & Hal1 & Hflr1)]"; wp_load; wp_store;
+        wp_store; wp_pures; iApply "Hphi". 
+        + iSplitR "Hlbs"; [|iLeft; by iFrame "Hlbs Hlv"]. 
+          iFrame. iFrame "Hal2 Hal4". iPureIntro; lia.
+        + iSplitR "Hlbs"; [|iLeft; by iFrame "Hlbs Hlv"]. 
+          iFrame "Hal2 Hal3 Hal4 Hun". iSplitR; [done|]. iSplitR; [done|].
+          iSplitR; [done|]. iSplitR "Hal1"; [iRight|iLeft]; by iFrame. } 
+    iApply "Hphi". iFrame. iSplitR; [iFrame "Hal2 Hal4"; iPureIntro; lia|].
     iLeft. iFrame "Hlbs". by iSplitR. 
   Qed.
 
